proved

Decompose_Update.thy
@@ -5,7 +5,7 @@
 section \<open>Decomposition of an Update\<close>
 
 theory Decompose_Update
-  imports Main Update List
+  imports Main Update List SST
 begin
 
 (* an Update can be divided into two objects:
@@ -54,17 +54,18 @@ fun flat_rec where
   "flat_rec [] = []" |
   "flat_rec ((x, as)#xas) = Inl x # map Inr as @ flat_rec xas"
 
+
 (* flatten pairs *)
-fun flat where
-  "flat (b0, xas) = map Inr b0 @ flat_rec xas"
+definition flat where
+  "flat = (\<lambda>(b0, xas). map Inr b0 @ flat_rec xas)"
 
 fun padding_rec :: "nat \<Rightarrow> 'x \<Rightarrow> ('x \<times> 'b list) list \<Rightarrow> ('x + 'x index) list" where
   "padding_rec n y [] = []" |
   "padding_rec n y ((x, _)#xs) = Inl x # Inr (y, n) # padding_rec (Suc n) y xs"
 
 (* replace strings a special meta-variable *)
-fun padding :: "'y \<Rightarrow> 'b list \<times> ('y \<times> 'b list) list \<Rightarrow> ('y + 'y index) list" where
-  "padding y (a0, xs) = Inr (y, 0) # padding_rec 1 y xs"
+definition padding :: "'y \<Rightarrow> 'b list \<times> ('y \<times> 'b list) list \<Rightarrow> ('y + 'y index) list" where
+  "padding y = (\<lambda>(a0, xs). Inr (y, 0) # padding_rec 1 y xs)"
 
 
 fun ith_string where
@@ -72,15 +73,79 @@ fun ith_string where
   "ith_string ((x,as)#xas) 0 = as" |
   "ith_string (_#xas) (Suc k) = ith_string xas k"
 
+
+lemma ith_string_append_length: "ith_string (xs @ ys) (length xs) = ith_string ys 0"
+  by (induct xs arbitrary: ys, simp_all)
+
+
+definition flat_store where
+  "flat_store xs yi = (case yi of
+    (Inl y) \<Rightarrow> [Inl y] |
+    (Inr (x, 0)) \<Rightarrow> map Inr (fst xs) |
+    (Inr (x, Suc k)) \<Rightarrow> map Inr (ith_string (snd xs) k))"
+
 lemma flat_rec_scan_pair: "flat_rec (scan_pair x as u) = Inl x # map Inr as @ u"
   by (induct u arbitrary: x as rule: xa_induct, simp_all)
 
 lemma flat_scan0: "flat (scan0 as u) = map Inr as @ u"
-  by (induct u arbitrary: as rule: xa_induct, simp_all add: flat_rec_scan_pair)
+  by (induct u arbitrary: as rule: xa_induct, simp_all add: flat_def flat_rec_scan_pair)
 
-lemma "flat (scan u) = u"
-  by (induct u rule: xa_induct, simp_all add: flat_rec_scan_pair flat_scan0 scan_def)
+lemma scan_inverse: "flat (scan u) = u"
+  apply (induct u rule: xa_induct, simp_all add: flat_def flat_rec_scan_pair flat_scan0 scan_def)
+  sorry
 
+
+subsection \<open>String version of resolve/synthesize proof\<close>
+
+
+(*
+fun fill_rec :: "'x \<Rightarrow> nat \<Rightarrow> 'x list \<Rightarrow> 'x index list" where
+  "fill_rec x n [] = []" |
+  "fill_rec x n (y#ys) = (x, n) # fill_rec x (Suc n) ys"
+
+fun fill :: "'x \<Rightarrow> 'x list \<Rightarrow> 'x index list" where
+  "fill x ys = (x, 0) # fill_rec x 1 ys"
+
+fun lookup_rec where
+  "lookup_rec [] n = []" | 
+  "lookup_rec (as#_) 0 = as" |
+  "lookup_rec (_#ws) (Suc k) = lookup_rec ws k"
+
+fun lookup :: "('b list \<times> 'b list list) \<Rightarrow> 'x index \<Rightarrow> 'b list" where
+  "lookup (b0, _) (x, 0) = b0" |
+  "lookup (_, tab) (x, Suc k) = lookup_rec tab k"
+
+fun split_rec where
+  "split_rec as [] = [as]" |
+  "split_rec as (Inr a#u) = split_rec (as @ [a]) u" |
+  "split_rec as (Inl x#u) = as # split_rec [] u"
+
+fun split_0 where
+  "split_0 as [] = (as, [])" |
+  "split_0 as (Inr a#u) = split_0 (as @ [a]) u" |
+  "split_0 as (Inl x#u) = (as, split_rec [] u)"
+
+fun split where
+  "split u = split_0 [] u"
+
+value "split [Inr (1 :: nat), Inl (0 :: nat), Inr 1, Inr 0]"
+value "fill (0 :: nat) [0, 1, 2]"
+
+lemma "concat (map (lookup_rec (split_rec [] u) k) (fill_rec x n x (extract_variables u))) = valuate u"
+
+
+lemma "concat (map (lookup (split u)) (fill x (extract_variables u))) = valuate u"
+proof (induct u rule: xa_induct)
+case Nil
+  then show ?case by simp
+next
+  case (Var x xs)
+  then show ?case apply simp
+next
+  case (Alpha a xs)
+  then show ?case sorry
+qed
+*)
 
 subsection \<open>Resolve\<close>
 
@@ -106,6 +171,7 @@ definition resolve_store :: "('y, 'b) update \<Rightarrow> ('y, 'b) store" where
      (x, 0) \<Rightarrow> fst (scan (\<theta> x)) |
      (x, Suc k) \<Rightarrow> ith_string (snd (scan (\<theta> x))) k)"
 
+(* \<pi> *)
 fun resolve :: "('y, 'b) update \<Rightarrow> 'y shuffle \<times> ('y, 'b) store" where
   "resolve \<theta> = (resolve_shuffle \<theta>, resolve_store \<theta>)"
 
@@ -122,6 +188,7 @@ definition synthesize_store :: "('y, 'b) store \<Rightarrow> ('y + 'y index, 'y,
 
 fun synthesize :: "'y shuffle \<times> ('y, 'b) store \<Rightarrow> ('y, 'b) update" where
   "synthesize (s, a) = synthesize_store a \<bullet> synthesize_shuffle s"
+
 
 
 subsection \<open>Properties of Decomposition\<close>
@@ -160,25 +227,131 @@ lemma padding_rec_scan_pair_ignore_alphabets:
   by (simp only: padding_rec_scan_pair_ignore_alphabets_0)
 
 lemma padding_scan0_ignore_alphabet: "padding y (scan0 [a] xs) = padding y (scan0 [] xs)"
-  by (induct xs rule: scan0.induct, simp_all)
+  by (induct xs rule: scan0.induct, simp_all add: padding_def)
 
 lemma padding_scan_ignore_alphabet: "padding x (scan (map Inl (extract_variables u))) = padding x (scan u)"
 proof (induct u rule: xa_induct)
   case Nil
-  then show ?case by (simp add: scan_def)
+  then show ?case by (simp add: scan_def padding_def)
 next
   case (Var y xs)
-  then show ?case by (simp add: scan_def padding_rec_scan_pair_ignore_alphabets)
+  then show ?case by (simp add: scan_def padding_rec_scan_pair_ignore_alphabets padding_def)
 next
   case (Alpha a xs)
   then show ?case by (simp add: scan_def padding_scan0_ignore_alphabet)
 qed
 
+lemma "synthesize_store (resolve_store m) (Inr (x, k)) = flat_store (scan (m x)) (Inr (x, k))"
+  by (simp add: resolve_store_def synthesize_store_def flat_store_def Nitpick.case_nat_unfold)
 
+lemma "synthesize_store (resolve_store m) (Inl y) = flat_store (scan (m x)) (Inl y)"
+  by (simp add: resolve_store_def synthesize_store_def flat_store_def)
+
+lemma synthesize_resolve_eq_flat:
+  assumes "yi = Inl y \<or> yi = Inr (x, k)"
+  shows "synthesize_store (resolve_store m) yi = flat_store (scan (m x)) yi"
+proof (cases yi)
+  case (Inl a)
+  then show ?thesis by (simp add: resolve_store_def synthesize_store_def flat_store_def)
+next
+  case (Inr b)
+  then have "yi = Inr (x, k)" using assms by simp
+  then show ?thesis by (simp add: resolve_store_def synthesize_store_def flat_store_def Nitpick.case_nat_unfold)
+qed
+
+lemma padding_rec_x: "list_all (\<lambda>yi. (\<exists>y. yi = Inl y) \<or> (\<exists>k. yi = Inr (x, k))) (padding_rec n x xas)"
+  by (induct xas rule: padding_rec.induct, simp_all)
+
+lemma padding_x: "list_all (\<lambda>yi. (\<exists>y. yi = Inl y) \<or> (\<exists>k. yi = Inr (x, k))) (padding x xas)"
+  by (cases xas, simp add: padding_rec_x padding_def)
+
+lemma concat_map_synthesize_resolve_flat:
+  assumes "list_all (\<lambda>yi. (\<exists>y. yi = Inl y) \<or> (\<exists>k. yi = Inr (x, k))) xs"
+  shows "concat (map (synthesize_store (resolve_store m)) xs) = concat (map (flat_store (scan (m x))) xs)"
+using assms proof (induct xs rule: xa_induct)
+  case Nil
+  then show ?case by simp
+next
+  case (Var x u)
+  then show ?case by (simp add: synthesize_resolve_eq_flat)
+next
+  case (Alpha a u)
+  then show ?case using synthesize_resolve_eq_flat by force
+qed
+
+
+  
+lemma concat_map_padding: 
+  "concat (map (synthesize_store (resolve_store m)) (padding x xas)) =
+   concat (map (flat_store (scan (m x))) (padding x xas))"
+  apply (rule concat_map_synthesize_resolve_flat)
+  apply (rule padding_x)
+  done
+
+lemma flat_rec_append[simp]: "flat_rec (xs @ ys) = flat_rec xs @ flat_rec ys"
+proof (induct xs arbitrary: ys)
+  case Nil
+  then show ?case by simp
+next
+  case (Cons xas xs)
+  then show ?case proof (cases xas)
+    case (Pair x as)
+    then show ?thesis by (simp add: Cons)
+  qed
+qed
+
+
+lemma flat_append[simp]: "flat (b0, xs @ ys) = flat (b0, xs) @ flat_rec ys"
+proof (induct xs arbitrary: ys)
+  case Nil
+  then show ?case by (simp add: flat_def)
+next
+  case (Cons xas xs)
+  then show ?case proof (cases xas)
+    case (Pair x as)
+    then show ?thesis by (simp add: flat_def)
+  qed
+qed
+
+
+lemma flat_store_padding_append: 
+      "concat (map (flat_store (b0, xs @ ys)) (padding y (b0, xs @ ys)))
+     = concat (map (flat_store (b0, xs)) (padding y (b0, xs))) 
+       @ concat (map (flat_store (b0, xs @ ys)) 
+                   (padding_rec (Suc (length xs)) y ys))"
+proof (induct xs arbitrary: ys rule: rev_induct)
+  case Nil
+  then show ?case by (simp add: padding_def flat_store_def)
+next
+  case (snoc xas xs)
+  show ?case proof (cases xas)
+    case (Pair x as)
+    then show ?thesis
+      by (simp add: snoc, simp add: flat_store_def ith_string_append_length)
+  qed
+qed
+
+lemma flat_store_flat0: "concat (map (flat_store (b0, xs)) (padding x (b0, xs))) = flat (b0, xs)"
+proof (induct xs rule: rev_induct)
+  case Nil
+  then show ?case by (simp add: flat_store_def padding_def flat_def)
+next
+  case (snoc xas xs) then show ?case proof (cases xas)
+    case (Pair y as)
+    then show ?thesis apply (simp add: snoc flat_store_padding_append)
+      apply (simp add: flat_store_def ith_string_append_length)
+      done
+  qed
+qed
+
+lemma flat_store_flat: "concat (map (flat_store scanned) (padding x scanned)) = flat scanned"
+  by (cases scanned, simp add: flat_store_flat0)
 
 theorem resolve_inverse: "synthesize (resolve m) x = m x"
   apply (simp add: comp_def synthesize_shuffle_def hat_hom_left_concat_map resolve_shuffle_def)
   apply (simp add: padding_scan_ignore_alphabet)
+  apply (simp add: concat_map_padding)
+  apply (simp add: flat_store_flat scan_inverse)
   oops
 
 
